<?xml version="1.0"?>
<rdf:RDF xmlns="https://w3id.org/def/odre-time#"
     xml:base="https://w3id.org/def/odre-time"
     xmlns:owl="http://www.w3.org/2002/07/owl#"
     xmlns:rdf="http://www.w3.org/1999/02/22-rdf-syntax-ns#"
     xmlns:xml="http://www.w3.org/XML/1998/namespace"
     xmlns:xsd="http://www.w3.org/2001/XMLSchema#"
     xmlns:rdfs="http://www.w3.org/2000/01/rdf-schema#"
     xmlns:terms="http://purl.org/dc/terms/">
    <owl:Ontology rdf:about="https://w3id.org/def/odre-time">
        <terms:creator>Andrea Cimmino</terms:creator>
        <terms:creator>Juan Cano de Benito</terms:creator>
        <terms:creator>http://www.garcia-castro.com/foaf.rdf#me</terms:creator>
        <rdfs:label>ODRL Time Extension</rdfs:label>
        <owl:versionInfo rdf:datatype="http://www.w3.org/2001/XMLSchema#decimal">1.0</owl:versionInfo>
    </owl:Ontology>
    


    <!-- 
    ///////////////////////////////////////////////////////////////////////////////////////
    //
    // Annotation properties
    //
    ///////////////////////////////////////////////////////////////////////////////////////
     -->


    


    <!-- http://purl.org/dc/terms/creator -->


    <owl:AnnotationProperty rdf:about="http://purl.org/dc/terms/creator"/>
    


    <!-- 
    ///////////////////////////////////////////////////////////////////////////////////////
    //
    // Classes
    //
    ///////////////////////////////////////////////////////////////////////////////////////
     -->


    


    <!-- http://www.semanticweb.org/juanc/ontologies/2024/7/untitled-ontology-37/between -->


    <owl:Class rdf:about="http://www.semanticweb.org/juanc/ontologies/2024/7/untitled-ontology-37/between">
        <rdfs:subClassOf rdf:resource="http://www.w3.org/ns/odrl/2/Operator"/>
        <rdfs:comment>A time given is between the Left Operand time and the Right Operand time</rdfs:comment>
    </owl:Class>
    


    <!-- http://www.semanticweb.org/juanc/ontologies/2024/7/untitled-ontology-37/time -->


    <owl:Class rdf:about="http://www.semanticweb.org/juanc/ontologies/2024/7/untitled-ontology-37/time">
        <rdfs:subClassOf rdf:resource="http://www.w3.org/ns/odrl/2/LeftOperand"/>
        <rdfs:subClassOf rdf:resource="http://www.w3.org/ns/odrl/2/RightOperand"/>
    </owl:Class>
    


    <!-- http://www.w3.org/2006/time#after -->


    <owl:Class rdf:about="http://www.w3.org/2006/time#after">
        <rdfs:subClassOf rdf:resource="http://www.w3.org/ns/odrl/2/Operator"/>
        <rdfs:comment>Left Operand time is after Right Operand time</rdfs:comment>
    </owl:Class>
    


    <!-- http://www.w3.org/2006/time#before -->


    <owl:Class rdf:about="http://www.w3.org/2006/time#before">
        <rdfs:subClassOf rdf:resource="http://www.w3.org/ns/odrl/2/Operator"/>
        <rdfs:comment>The time provided by the left operand side occurs before the time on the right operand side.</rdfs:comment>
    </owl:Class>
    


    <!-- http://www.w3.org/2006/time#contains -->


    <owl:Class rdf:about="http://www.w3.org/2006/time#contains">
        <rdfs:subClassOf rdf:resource="http://www.w3.org/ns/odrl/2/Operator"/>
        <rdfs:comment>The right operand event occurs entirely within the duration of the left operand event.</rdfs:comment>
    </owl:Class>
    


    <!-- http://www.w3.org/2006/time#during -->


    <owl:Class rdf:about="http://www.w3.org/2006/time#during">
        <rdfs:subClassOf rdf:resource="http://www.w3.org/ns/odrl/2/Operator"/>
        <rdfs:comment>The left operand event occurs entirely within the duration of the right operand event.</rdfs:comment>
    </owl:Class>
    


    <!-- http://www.w3.org/2006/time#equals -->


    <owl:Class rdf:about="http://www.w3.org/2006/time#equals">
        <rdfs:subClassOf rdf:resource="http://www.w3.org/ns/odrl/2/Operator"/>
        <rdfs:comment>The events on the left operand and right operand side have exactly the same duration and occur at the same time.</rdfs:comment>
    </owl:Class>
    


    <!-- http://www.w3.org/2006/time#finished -->


    <owl:Class rdf:about="http://www.w3.org/2006/time#finished">
        <rdfs:subClassOf rdf:resource="http://www.w3.org/ns/odrl/2/Operator"/>
        <rdfs:comment>The event on the left operand ends at exactly the same time as the event on the right operand.</rdfs:comment>
    </owl:Class>
    


    <!-- http://www.w3.org/2006/time#finishedBy -->


    <owl:Class rdf:about="http://www.w3.org/2006/time#finishedBy">
        <rdfs:subClassOf rdf:resource="http://www.w3.org/ns/odrl/2/Operator"/>
        <rdfs:comment>The event on the right operand ends at exactly the same time as the event on the left operand.</rdfs:comment>
    </owl:Class>
    


    <!-- http://www.w3.org/2006/time#meets -->


    <owl:Class rdf:about="http://www.w3.org/2006/time#meets">
        <rdfs:subClassOf rdf:resource="http://www.w3.org/ns/odrl/2/Operator"/>
        <rdfs:comment>The end of the event or object on the left operand coincides exactly with the start of the event on the right operand.</rdfs:comment>
    </owl:Class>
    


    <!-- http://www.w3.org/2006/time#metBy -->


    <owl:Class rdf:about="http://www.w3.org/2006/time#metBy">
        <rdfs:subClassOf rdf:resource="http://www.w3.org/ns/odrl/2/Operator"/>
        <rdfs:comment>The end of the event or object on the right operand coincides exactly with the start of the event on the left operand.</rdfs:comment>
    </owl:Class>
    


    <!-- http://www.w3.org/2006/time#overlappedBy -->


    <owl:Class rdf:about="http://www.w3.org/2006/time#overlappedBy">
        <rdfs:subClassOf rdf:resource="http://www.w3.org/ns/odrl/2/Operator"/>
        <rdfs:comment>The event on the right operand starts before the event on the left operand, but also ends before the event on the left operand ends.</rdfs:comment>
    </owl:Class>
    


    <!-- http://www.w3.org/2006/time#overlaps -->


    <owl:Class rdf:about="http://www.w3.org/2006/time#overlaps">
        <rdfs:subClassOf rdf:resource="http://www.w3.org/ns/odrl/2/Operator"/>
        <rdfs:comment>The event on the left operand starts before the event on the right operand, but also ends before the event on the right operand ends.</rdfs:comment>
    </owl:Class>
    


    <!-- http://www.w3.org/2006/time#startedBy -->


    <owl:Class rdf:about="http://www.w3.org/2006/time#startedBy">
        <rdfs:subClassOf rdf:resource="http://www.w3.org/ns/odrl/2/Operator"/>
        <rdfs:comment>The event on the right operand starts at exactly the same time as the event on the left operand.</rdfs:comment>
    </owl:Class>
    


    <!-- http://www.w3.org/2006/time#starts -->


    <owl:Class rdf:about="http://www.w3.org/2006/time#starts">
        <rdfs:subClassOf rdf:resource="http://www.w3.org/ns/odrl/2/Operator"/>
        <rdfs:comment>The event on the left operand starts at exactly the same time as the event on the right operand.</rdfs:comment>
    </owl:Class>
    


    <!-- http://www.w3.org/ns/odrl/2/LeftOperand -->


    <owl:Class rdf:about="http://www.w3.org/ns/odrl/2/LeftOperand"/>
    


    <!-- http://www.w3.org/ns/odrl/2/Operator -->


    <owl:Class rdf:about="http://www.w3.org/ns/odrl/2/Operator"/>
    


    <!-- http://www.w3.org/ns/odrl/2/RightOperand -->


    <owl:Class rdf:about="http://www.w3.org/ns/odrl/2/RightOperand"/>
</rdf:RDF>



<!-- Generated by the OWL API (version 5.1.18) https://github.com/owlcs/owlapi/ -->


