@prefix : <https://w3id.org/def/odre-time#> .
@prefix owl: <http://www.w3.org/2002/07/owl#> .
@prefix rdf: <http://www.w3.org/1999/02/22-rdf-syntax-ns#> .
@prefix xml: <http://www.w3.org/XML/1998/namespace> .
@prefix xsd: <http://www.w3.org/2001/XMLSchema#> .
@prefix rdfs: <http://www.w3.org/2000/01/rdf-schema#> .
@base <https://w3id.org/def/odre-time#> .

<https://w3id.org/def/odre-time> rdf:type owl:Ontology ;
                                  <http://purl.org/dc/terms/creator> "Andrea Cimmino" ,
                                                                     "Juan Cano de Benito" ,
                                                                     "http://www.garcia-castro.com/foaf.rdf#me" ;
                                  rdfs:label "ODRL Time Extension" ;
                                  owl:versionInfo 1.0 .

#################################################################
#    Annotation properties
#################################################################

###  http://purl.org/dc/terms/creator
<http://purl.org/dc/terms/creator> rdf:type owl:AnnotationProperty .


#################################################################
#    Classes
#################################################################

###  http://www.semanticweb.org/juanc/ontologies/2024/7/untitled-ontology-37/between
<http://www.semanticweb.org/juanc/ontologies/2024/7/untitled-ontology-37/between> rdf:type owl:Class ;
                                                                                  rdfs:subClassOf <http://www.w3.org/ns/odrl/2/Operator> ;
                                                                                  rdfs:comment "A time given is between the Left Operand time and the Right Operand time" .


###  http://www.semanticweb.org/juanc/ontologies/2024/7/untitled-ontology-37/time
<http://www.semanticweb.org/juanc/ontologies/2024/7/untitled-ontology-37/time> rdf:type owl:Class ;
                                                                               rdfs:subClassOf <http://www.w3.org/ns/odrl/2/LeftOperand> ,
                                                                                               <http://www.w3.org/ns/odrl/2/RightOperand> .


###  http://www.w3.org/2006/time#after
<http://www.w3.org/2006/time#after> rdf:type owl:Class ;
                                    rdfs:subClassOf <http://www.w3.org/ns/odrl/2/Operator> ;
                                    rdfs:comment "Left Operand time is after Right Operand time" .


###  http://www.w3.org/2006/time#before
<http://www.w3.org/2006/time#before> rdf:type owl:Class ;
                                     rdfs:subClassOf <http://www.w3.org/ns/odrl/2/Operator> ;
                                     rdfs:comment "The time provided by the left operand side occurs before the time on the right operand side." .


###  http://www.w3.org/2006/time#contains
<http://www.w3.org/2006/time#contains> rdf:type owl:Class ;
                                       rdfs:subClassOf <http://www.w3.org/ns/odrl/2/Operator> ;
                                       rdfs:comment "The right operand event occurs entirely within the duration of the left operand event." .


###  http://www.w3.org/2006/time#during
<http://www.w3.org/2006/time#during> rdf:type owl:Class ;
                                     rdfs:subClassOf <http://www.w3.org/ns/odrl/2/Operator> ;
                                     rdfs:comment "The left operand event occurs entirely within the duration of the right operand event." .


###  http://www.w3.org/2006/time#equals
<http://www.w3.org/2006/time#equals> rdf:type owl:Class ;
                                     rdfs:subClassOf <http://www.w3.org/ns/odrl/2/Operator> ;
                                     rdfs:comment "The events on the left operand and right operand side have exactly the same duration and occur at the same time." .


###  http://www.w3.org/2006/time#finished
<http://www.w3.org/2006/time#finished> rdf:type owl:Class ;
                                       rdfs:subClassOf <http://www.w3.org/ns/odrl/2/Operator> ;
                                       rdfs:comment "The event on the left operand ends at exactly the same time as the event on the right operand." .


###  http://www.w3.org/2006/time#finishedBy
<http://www.w3.org/2006/time#finishedBy> rdf:type owl:Class ;
                                         rdfs:subClassOf <http://www.w3.org/ns/odrl/2/Operator> ;
                                         rdfs:comment "The event on the right operand ends at exactly the same time as the event on the left operand." .


###  http://www.w3.org/2006/time#meets
<http://www.w3.org/2006/time#meets> rdf:type owl:Class ;
                                    rdfs:subClassOf <http://www.w3.org/ns/odrl/2/Operator> ;
                                    rdfs:comment "The end of the event or object on the left operand coincides exactly with the start of the event on the right operand." .


###  http://www.w3.org/2006/time#metBy
<http://www.w3.org/2006/time#metBy> rdf:type owl:Class ;
                                    rdfs:subClassOf <http://www.w3.org/ns/odrl/2/Operator> ;
                                    rdfs:comment "The end of the event or object on the right operand coincides exactly with the start of the event on the left operand." .


###  http://www.w3.org/2006/time#overlappedBy
<http://www.w3.org/2006/time#overlappedBy> rdf:type owl:Class ;
                                           rdfs:subClassOf <http://www.w3.org/ns/odrl/2/Operator> ;
                                           rdfs:comment "The event on the right operand starts before the event on the left operand, but also ends before the event on the left operand ends." .


###  http://www.w3.org/2006/time#overlaps
<http://www.w3.org/2006/time#overlaps> rdf:type owl:Class ;
                                       rdfs:subClassOf <http://www.w3.org/ns/odrl/2/Operator> ;
                                       rdfs:comment "The event on the left operand starts before the event on the right operand, but also ends before the event on the right operand ends." .


###  http://www.w3.org/2006/time#startedBy
<http://www.w3.org/2006/time#startedBy> rdf:type owl:Class ;
                                        rdfs:subClassOf <http://www.w3.org/ns/odrl/2/Operator> ;
                                        rdfs:comment "The event on the right operand starts at exactly the same time as the event on the left operand." .


###  http://www.w3.org/2006/time#starts
<http://www.w3.org/2006/time#starts> rdf:type owl:Class ;
                                     rdfs:subClassOf <http://www.w3.org/ns/odrl/2/Operator> ;
                                     rdfs:comment "The event on the left operand starts at exactly the same time as the event on the right operand." .


###  http://www.w3.org/ns/odrl/2/LeftOperand
<http://www.w3.org/ns/odrl/2/LeftOperand> rdf:type owl:Class .


###  http://www.w3.org/ns/odrl/2/Operator
<http://www.w3.org/ns/odrl/2/Operator> rdf:type owl:Class .


###  http://www.w3.org/ns/odrl/2/RightOperand
<http://www.w3.org/ns/odrl/2/RightOperand> rdf:type owl:Class .


###  Generated by the OWL API (version 5.1.18) https://github.com/owlcs/owlapi/
